Starting on docs

Total/Stlc/Lang/Surface/Grammar.lean
@@ -1,31 +1,98 @@
 set_option autoImplicit false
 
 namespace Total.Stlc.Lang.Surface
+  /-!
+  # Simply-Typed Lambda Calculus Surface Syntax Grammar
+
+  These are the inductive types defined for representing terms of the surface
+  syntax.
+  -/
+
+  /--
+  # Types
+
+  Representation of types.
+  -/
   inductive Ty: Type where
+     /-- Booleans -/
     | bool: Ty
+    /-- Natural Numbers -/
     | nat: Ty
 
+  /--
+  # Unary Operators
+
+  The supported unary operators.
+
+  These are bare operators and unary operator expressions.  The representation
+  of the latter is in the type for `Term`s.
+  -/
   inductive UnOp: Type where
+    /-- Logical Negation -/
     | not: UnOp
 
+  /--
+  # Binary Operators
+
+  The supported binary operators.
+
+  These are bare operators and binary operator expressions.  The representation
+  of the latter is in the type for `Term`s.
+  -/
   inductive BinOp: Type where
+    /-- Logical Conjunction (AND) -/
     | and: BinOp
+    /-- Logical Disjunction (OR) -/
     | or:  BinOp
+    /-- Addition -/
     | add: BinOp
+    /-- Multiplication -/
     | mul: BinOp
+    /-- Boolean Equality -/
     | eq:  BinOp
+    /-- Boolean Inequality -/
     | neq: BinOp
+    /-- Less Than -/
     | lt:  BinOp
+    /-- Less Than or Equal -/
     | lte: BinOp
+    /-- Greater Than -/
     | gt:  BinOp
+    /-- Greater Than or Equal -/
     | gte: BinOp
 
+  /--
+  # Terms
+
+  Terms of the language.
+  -/
   inductive Term: Type where
+    /-- Boolean literal -/
     | bool (b: Bool): Term
+    /-- Natural number literal -/
     | nat  (n: Nat): Term
+    /-- Unary operator application -/
     | unOp (op: UnOp) (operand: Term): Term
+    /-- Binary operator application -/
     | binOp (op: BinOp) (lhs rhs: Term): Term
+    /-- Conditional expression -/
     | cond (c t f: Term): Term
 
+  /--
+  # Top-Level Terms
+
+  Top-level terms of the language.
+  -/
   inductive Top: Type where
+
+  /--
+  # Files
+
+  Source files.
+  -/
+  structure File: Type where
+    /--
+    The top-level terms in the file, in the order present in the file.
+    -/
+    tops: List Top
 namespace Total.Stlc.Lang.Surface
