Total/Stlc/Lang/Surface/Termination.lean
@@ -7,49 +7,120 @@ import Total.Stlc.Lang.Surface.Semantics
 set_option autoImplicit false
 
 namespace Total.Stlc.Lang.Surface
+  /-!
+  # Simply-Typed Lambda Calculus Surface Syntax Termination Semantics
+
+  These are the termination-specific semantics of the language.
+
+  These are separate from the main semantics of the language as they are defined
+  in terms of those main semantics.
+  -/
+
   namespace UnOp
+/-!
+# Unary Operators
+-/
+
     variable {τ₁ τ₂: Ty}
     variable {op: UnOp}
-    variable {t: Term}
+    variable {operand: Term}
 
-    @[reducible]
-    def Halts (op: UnOp) (t₁: Term): Prop := ∃ t₂: Term, Eval₁ op t₁ t₂ ∧ Term.IsValue t₂
+    /--
+    ## Halts
 
+    A unary operator `op` halts when applied to an operand `operand₁` if the
+    application evaluates to a value `operand₂`.
+    -/
     @[reducible]
-    def Total (τ₁ τ₂: Ty) (op: UnOp) (t: Term): Prop :=
-      (HasType op τ₁ τ₂) ∧ (Halts op t) ∧ True
+    def Halts (op: UnOp) (operand₁: Term): Prop := ∃ operand₂: Term, Eval₁ op operand₁ operand₂ ∧ Term.IsValue operand₂
+
+    /--
+    ## Totality
+
+    A unary operator `op` that takes operands of type `τ₁` and produces results
+    of type `τ₂` is total when applied to `operand` if the application halts.
+    -/
+    @[reducible]
+    def Total (τ₁ τ₂: Ty) (op: UnOp) (operand: Term): Prop :=
+      (HasType op τ₁ τ₂) ∧ (Halts op operand)
 
     namespace Total
-      theorem halts: Total τ₁ τ₂ op t → Halts op t
-        | ⟨_, hh, _⟩ => hh
+/-!
+## Termination of Total Unary Operations
+-/
+
+      /--
+      Total unary operator applications halt.
+      -/
+      theorem halts: Total τ₁ τ₂ op operand → Halts op operand
+        | ⟨_, hh⟩ => hh
     end Total
   end UnOp
 
   namespace BinOp
+/-!
+# Binary Operators
+-/
     variable {τ₁ τ₂ τ₃: Ty}
     variable {op: BinOp}
-    variable {t₁ t₂: Term}
+    variable {lhs rhs: Term}
 
-    @[reducible]
-    def Halts (op: BinOp) (t₁ t₂: Term): Prop := ∃ t₃: Term, Eval₁ op t₁ t₂ t₃ ∧ Term.IsValue t₃
+    /--
+    ## Halts
 
+    A binary operator `op` halts when applied to left- and right-hand operands
+    `lhs` and `rhs` if the application evaluates to a value `res`.
+    -/
     @[reducible]
-    def Total (τ₁ τ₂ τ₃: Ty) (op: BinOp) (t₁ t₂: Term): Prop :=
-      (HasType op τ₁ τ₂ τ₃) ∧ (Halts op t₁ t₂) ∧ True
+    def Halts (op: BinOp) (lhs rhs: Term): Prop := ∃ res: Term, Eval₁ op lhs rhs res ∧ Term.IsValue res
+
+    /--
+    ## Totality
+
+    A binary operator `op` that takes operands of type `τ₁` and `τ₂` and
+    produces results of type `τ₃` is total when applied to left- and right-hand
+    operands `lhs` and `rhs` if the application halts.
+    -/
+    @[reducible]
+    def Total (τ₁ τ₂ τ₃: Ty) (op: BinOp) (lhs rhs: Term): Prop :=
+      (HasType op τ₁ τ₂ τ₃) ∧ (Halts op lhs rhs)
 
     namespace Total
-      theorem halts: Total τ₁ τ₂ τ₃ op t₁ t₂ → Halts op t₁ t₂
-        | ⟨_, hh, _⟩ => hh
+/-!
+## Termination of Total Binary Operations
+-/
+
+      /--
+      Total binary operator applications halt.
+      -/
+      theorem halts: Total τ₁ τ₂ τ₃ op lhs rhs → Halts op lhs rhs
+        | ⟨_, hh⟩ => hh
     end Total
   end BinOp
 
   namespace Term
+/-!
+# Terms
+-/
     variable {τ: Ty}
     variable {t: Term}
 
+    /--
+    ## Halts
+
+    A term `t₁` halts if it evaluates to a value `t₂`.
+    -/
     @[reducible]
     def Halts (t₁: Term): Prop := ∃ t₂: Term, Eval t₁ t₂ ∧ IsValue t₂
 
+    /--
+    ## Totality
+
+    A term `t` of type `τ` is total if it halts and one of the following:
+
+    - It is of type boolean
+    - It is of type nat
+    -/
     @[reducible]
     def Total (τ: Ty) (t: Term): Prop :=
       (HasType t τ) ∧ (Halts t) ∧ (
@@ -59,12 +130,26 @@ namespace Total.Stlc.Lang.Surface
       )
 
     namespace IsValue
+/-!
+## Termination of Values
+-/
+
+      /--
+      Values halt.
+      -/
       theorem halts: IsValue t → Halts t
         | .bool _ => ⟨_, .refl, .bool _⟩
         | .nat  _ => ⟨_, .refl, .nat  _⟩
     end IsValue
 
     namespace Total
+/-!
+## Termination of Total Terms
+-/
+
+      /--
+      Total terms halt.
+      -/
       theorem halts: {t: Term} → Total τ t → Halts t
         | .bool  _,     _                   => IsValue.halts (.bool _)
         | .nat   _,     _                   => IsValue.halts (.nat  _)
@@ -77,22 +162,61 @@ namespace Total.Stlc.Lang.Surface
   end Term
 
   namespace Top
+/-!
+# Top-Level Terms
+-/
+
     variable {τ: Ty}
     variable {t: Top}
 
+    /--
+    ## Halts
+
+    A top-level term `t₁` halts if it evaluates to a value `t₂`.
+    -/
     @[reducible]
     def Halts (t₁: Top): Prop := ∃ t₂: Top, Eval t₁ t₂ ∧ IsValue t₂
 
+    /--
+    ## Totality
+
+    A top-level term `t` of type `τ` is total if it halts and one of the
+    following:
+
+    - It is of type boolean
+    - It is of type nat
+    -/
     @[reducible]
     def Total: Ty → Top → Prop
       | .bool, t => nomatch t
 
     namespace IsValue
+/-!
+## Termination of Values
+-/
+
+      /--
+      Values halt.
+      -/
       theorem halts: IsValue t → Halts t := nomatch t
     end IsValue
 
     namespace Total
+/-!
+## Termination of Total Terms
+-/
+
+      /--
+      Total terms halt.
+      -/
       theorem halts {t: Top}: Total τ t → Halts t := nomatch t
     end Total
   end Top
+
+  namespace File
+/-!
+# Files
+-/
+
+  end File
 end Total.Stlc.Lang.Surface
