Total/Stlc/Lang/Surface/Semantics.lean
@@ -6,76 +6,496 @@ import Total.Stlc.Lang.Surface.Syntax
 set_option autoImplicit false
 
 namespace Total.Stlc.Lang.Surface
-  section Types
-  end Types
+  /-!
+  # Simply-Typed Lambda Calculus Surface Syntax Semantics
+
+  These are the semantics of the language, given as inductive relations.
+  -/
 
   namespace UnOp
+/-!
+# Unary Operators
+
+Unary operators are primitive operations that operate on a single value
+operand and produce a value result.  The type of the operand and the result
+are not necessarily the same.
+
+## Implemented Operators
+
+There is one group of operators currently supported:
+
+- **Logical**: Negation of boolean values (logical NOT)
+
+The common operation of arithmetic negation is not supported as it is not
+closed in the natural numbers.
+-/
+
+    /--
+    ## Typing Relation
+
+    The typing relation contains the allowed typing derevations for unary
+    operators.
+
+    ### Indexes
+
+    The typing relation is indexed by three values:
+
+    - The operator
+    - The type of the operand
+    - The type of the result
+    -/
     inductive HasType: UnOp → Ty → Ty → Prop where
+      /-- Logical Negation maps from Boolean values to Boolean values -/
       | not: HasType .not [Ty| 𝔹] [Ty| 𝔹]
 
+    /--
+    ## Single-Step Evaluation Relation
+
+    The single-step evaluation relation contains all of the terms that can be
+    computed in a single step by a unary operator.
+
+    The inference rules in this relation take primitive Lean values instead of
+    `Term`s since these are primitive operations that require their operand to
+    be a value.  The rules for reducing the operand to a value are in the
+    single-step evaluation relation for `Term`s.
+
+    ### Indexes
+
+    The single-step evaluation relation is indexed by three values:
+
+    - The operator
+    - The operand
+    - The result
+    -/
     inductive Eval₁: UnOp → Term → Term → Prop where
+      /--
+      Logical Negation takes a boolean `operand` and performs a logical `not` on
+      it.
+      -/
       | not {operand: Bool}: Eval₁ .not (.bool operand) (.bool !operand)
   end UnOp
 
   namespace BinOp
+/-!
+# Binary Operators
+
+Unary operators are primitive operations that operate on two value
+operands (a left-hand and a right-hand operand) and produce a value result.
+The types of the left- and right-hand operands and the result are not
+necessarily the same.
+
+## Implemented Operators
+
+There are four groups of operators currently supported:
+
+- **Logical**: Conjuction and disjunction of boolean values (logical AND and
+  logical OR)
+- **Arithmetic**: Addition and multiplication of natural numbers.  These
+  operations are supported because they are closed in the natural numbers,
+  whereas the commonly included Subtraction, division, and modulus are not.
+- **Equality**: Equals and Not Equals.  These operators are inherently
+  polymorphic and are supported on both Boolean and Natural number values.
+- **Comparison**: Less Than- and Greater Than- (or Equals) operators that
+  compare natural numbers.
+-/
+
+    /--
+    ## Typing Relation
+
+    The typing relation contains the allowed typing derevations for binary
+    operators.
+
+    ### Indexes
+
+    The typing relation is indexed by four values:
+
+    - The operator
+    - The type of the left-hand operand
+    - The type of the right-hand operand
+    - The type of the result
+    -/
     inductive HasType: BinOp → Ty → Ty → Ty → Prop
+      /--
+      Logical Conjunction operates on Boolean inputs and produces a Boolean
+      result.
+      -/
       | and: HasType .and [Ty| 𝔹] [Ty| 𝔹] [Ty| 𝔹]
+      /--
+      Logical Disjunction operates on Boolean inputs and produces a Boolean
+      result.
+      -/
       | or:  HasType .or  [Ty| 𝔹] [Ty| 𝔹] [Ty| 𝔹]
+      /--
+      Addition operates on Nat inputs and produces a Nat result.
+      -/
       | add: HasType .add [Ty| ℕ] [Ty| ℕ] [Ty| ℕ]
+      /--
+      Multiplication operates on Nat inputs and produces a Nat result.
+      -/
       | mul: HasType .mul [Ty| ℕ] [Ty| ℕ] [Ty| ℕ]
+      /--
+      Equality operates on inputs with identical types and produces a Boolean
+      result.
+      -/
       | eq  {τ: Ty}: HasType .eq  [Ty| ‹τ›] [Ty| ‹τ›] [Ty| 𝔹]
+      /--
+      Inequality operates on inputs with identical types and produces a Boolean
+      result.
+      -/
       | neq {τ: Ty}: HasType .neq [Ty| ‹τ›] [Ty| ‹τ›] [Ty| 𝔹]
+      /--
+      Less Than operates on Nat inputs and produces a Boolean result.
+      -/
       | lt:  HasType .lt  [Ty| ℕ] [Ty| ℕ] [Ty| 𝔹]
+      /--
+      Less Than or Equal operates on Nat inputs and produces a Boolean result.
+      -/
       | lte: HasType .lte [Ty| ℕ] [Ty| ℕ] [Ty| 𝔹]
+      /--
+      Greater Than operates on Nat inputs and produces a Boolean result.
+      -/
       | gt:  HasType .gt  [Ty| ℕ] [Ty| ℕ] [Ty| 𝔹]
+      /--
+      Greater Than or Equal operates on Nat inputs and produces a Boolean
+      result.
+      -/
       | gte: HasType .gte [Ty| ℕ] [Ty| ℕ] [Ty| 𝔹]
 
+    /--
+    ## Single-Step Evaluation Relation
+
+    The single-step evaluation relation contains all of the terms that can be
+    computed in a single step by a binary operator.
+
+    The inference rules in this relation take primitive Lean values instead of
+    `Term`s since these are primitive operations that require their operands to
+    be values.  The rules for reducing the operands to values are in the
+    single-step evaluation relation for `Term`s.
+
+    ### Indexes
+
+    The single-step evaluation relation is indexed by four values:
+
+    - The operator
+    - The left-hand operand
+    - The right-hand operand
+    - The result
+    -/
     inductive Eval₁: BinOp → Term → Term → Term → Prop where
+      /--
+      Logical Conjuction takes two boolean values `lhs` and `rhs` and returns
+      `lhs && rhs`.
+      -/
       | and {lhs rhs: Bool}: Eval₁ .and [Term| ‹bool:lhs›] [Term| ‹bool:rhs›] [Term| ‹bool:lhs && rhs›]
+      /--
+      Logical Disjunction takes two boolean values `lhs` and `rhs` and returns
+      `lhs || rhs`.
+      -/
       | or  {lhs rhs: Bool}: Eval₁ .or  [Term| ‹bool:lhs›] [Term| ‹bool:rhs›] [Term| ‹bool:lhs || rhs›]
+      /--
+      Addition takes two natural number values `lhs` and `rhs` and returns their
+      sum (`lhs + rhs`).
+      -/
       | add {lhs rhs: Nat}:  Eval₁ .add [Term| ‹nat:lhs›]  [Term| ‹nat:rhs›]  [Term| ‹nat:lhs + rhs›]
+      /--
+      Multiplication takes two natural number values `lhs` and `rhs` and returns their
+      product (`lhs * rhs`).
+      -/
       | mul {lhs rhs: Nat}:  Eval₁ .mul [Term| ‹nat:lhs›]  [Term| ‹nat:rhs›]  [Term| ‹nat:lhs * rhs›]
+      /--
+      Boolean equality takes two boolean values `lhs` and `rhs` and returns
+      `true` if they are equal and `false` otherwise (`lhs == rhs`).
+      -/
       | eqBool  {lhs rhs: Bool}: Eval₁ .eq  [Term| ‹bool:lhs›] [Term| ‹bool:rhs›] [Term| ‹bool:lhs == rhs›]
+      /--
+      Natural number equality takes two natural number values `lhs` and `rhs` and
+      returns `true` if they are equal and `false` otherwise (`lhs == rhs`).
+      -/
       | eqNat   {lhs rhs: Nat}:  Eval₁ .eq  [Term| ‹nat:lhs›]  [Term| ‹nat:rhs›]  [Term| ‹bool:lhs == rhs›]
+      /--
+      Boolean inequality takes two boolean values `lhs` and `rhs` and returns
+      `true` if they are unequal and `false` otherwise (`lhs != rhs`).
+      -/
       | neqBool {lhs rhs: Bool}: Eval₁ .neq [Term| ‹bool:lhs›] [Term| ‹bool:rhs›] [Term| ‹bool:lhs != rhs›]
+      /--
+      Natural number inequality takes two natural number values `lhs` and `rhs`
+      and returns `true` if they are unequal and `false` otherwise
+      (`lhs != rhs`).
+      -/
       | neqNat  {lhs rhs: Nat}:  Eval₁ .neq [Term| ‹nat:lhs›]  [Term| ‹nat:rhs›]  [Term| ‹bool:lhs != rhs›]
+      /--
+      Less than comparison takes two natural number values `lhs` and `rhs` and
+      returns `true` if the first is less than the second (`lhs < rhs`).
+      -/
       | lt  {lhs rhs: Nat}: Eval₁ .lt  [Term| ‹nat:lhs›] [Term| ‹nat:rhs›] [Term| ‹bool:lhs < rhs›]
+      /--
+      Less than or equal comparison takes two natural number values `lhs` and
+      `rhs` and returns `true` if the first is less than or equal to the second
+      (`lhs ≤ rhs`).
+      -/
       | lte {lhs rhs: Nat}: Eval₁ .lte [Term| ‹nat:lhs›] [Term| ‹nat:rhs›] [Term| ‹bool:lhs ≤ rhs›]
+      /--
+      Greater than comparison takes two natural number values `lhs` and `rhs`
+      and returns `true` if the first is greater than the second (`lhs > rhs`).
+      -/
       | gt  {lhs rhs: Nat}: Eval₁ .gt  [Term| ‹nat:lhs›] [Term| ‹nat:rhs›] [Term| ‹bool:lhs > rhs›]
+      /--
+      Greater than or equal comparison takes two natural number values `lhs` and
+      `rhs` and returns `true` if the first is greater than or equal to the
+      second (`lhs ≥ rhs`).
+      -/
       | gte {lhs rhs: Nat}: Eval₁ .gte [Term| ‹nat:lhs›] [Term| ‹nat:rhs›] [Term| ‹bool:lhs ≥ rhs›]
   end BinOp
 
   namespace Term
+/-!
+# Terms
+-/
+
+    /--
+    ## Value Relation
+
+    The value relation contains the terms that are values, i.e., terms that
+    cannot be reduced any further by the evaluation rules.
+
+    ### Indexes
+
+    The value relation is indexed by one value:
+
+    - The term
+    -/
     inductive IsValue: Term → Prop where
+      /-- Boolean literals are values -/
       | bool (b: Bool): IsValue [Term| ‹bool:b›]
+      /-- Natural number literals are values -/
       | nat (n: Nat): IsValue [Term| ‹nat:n›]
 
+    /--
+    ## Typing Relation
+
+    The typing relation contains the allowed typing derivations for terms.
+
+    ### Indexes
+
+    The value relation is indexed by two values:
+
+    - The term
+    - The term's derived type
+    -/
     inductive HasType: Term → Ty → Prop where
+      /-- Boolean literals are of Boolean type -/
       | bool {b: Bool}: HasType [Term| ‹bool:b›] [Ty| 𝔹]
+      /-- Natural number literals are of Nat type -/
       | nat {n: Nat}: HasType [Term| ‹nat:n›] [Ty| ℕ]
+      /--
+      Unary operation expressions have the type of their result (`τ₂`).
+
+      ### Premises
+
+      - `h₁`: The unary operator maps from an input of type `τ₁` to a result of
+        type `τ₂`
+      - `h₂`: The operand has type `τ₁`.
+
+      ### Conclusion
+
+      The unary operator expression has type `τ₂`.
+      -/
       | unOp {τ₁ τ₂: Ty} {op: UnOp} {operand: Term} (h₁: UnOp.HasType op τ₁ τ₂) (h₂: HasType operand τ₁): HasType (.unOp op operand) τ₂
+      /--
+      Binary operation expressions have the type of their result (`τ₃`).
+
+      ### Premises
+
+      - `h₁`: The binary operator maps from inputs of type `τ₁` and `τ₂` to a
+        result of type `τ₃`
+      - `h₂`: The left-hand side operand has type `τ₁`.
+      - `h₃`: The left-hand side operand has type `τ₂`.
+
+      ### Conclusion
+
+      The binary operator expression has type `τ₃`.
+      -/
       | binOp {τ₁ τ₂ τ₃: Ty} {op: BinOp} {lhs rhs: Term} (h₁: BinOp.HasType op τ₁ τ₂ τ₃) (h₂: HasType lhs τ₁) (h₃: HasType rhs τ₂): HasType (.binOp op lhs rhs) τ₃
+      /--
+      Conditional expressions have the type of their `then` and `else` clauses.
+      The types of the clauses must be equal.
+
+      ### Premises
+
+      - `h₁`: The condition is of Boolean type
+      - `h₂`: The `then` clause has some type `τ`.
+      - `h₃`: The `else` clause has the same type `τ`.
+
+      ### Conclusion
+
+      The conditional operator expression has type `τ`.
+      -/
       | cond {c t f: Term} {τ: Ty} (h₁: HasType c [Ty| 𝔹]) (h₂: HasType t τ) (h₃: HasType f τ): HasType [Term| if ‹c› then ‹t› else ‹f›] τ
 
+    /--
+    ## Single-Step Evaluation Relation
+
+    The single-step evaluation relation contains all of the terms that can be
+    computed in a single step.
+
+    ### Indexes
+
+    The value relation is indexed by two values:
+
+    - The term being evaluated
+    - The term it evaluates to
+    -/
     inductive Eval₁: Term → Term → Prop where
+      /--
+      Unary operators applied to a value operand follow the unary operator
+      single-step semantics.
+
+      ### Premises
+
+      - `h₁`: The operand is a value
+      - `h₂`: A single-step unary operation evaluation
+
+      ### Conclusion
+
+      The term evaluates to the result of the unary operation evaluation.
+      -/
       | unOp {op: UnOp} {operand res: Term} (h₁: IsValue operand) (h₂: UnOp.Eval₁ op operand res): Eval₁ (.unOp op operand) res
+      /--
+      Unary operators applied to a non-value operand evaluate the operand using
+      the term single-step semantics.
+
+      ### Premises
+
+      - `h`: A single-step term evaluation of the operand
+
+      ### Conclusion
+
+      The operand takes an evaluation step.
+      -/
       | unOpOp {op: UnOp} {operand₁ operand₂: Term} (h: Eval₁ operand₁ operand₂): Eval₁ (.unOp op operand₁) (.unOp op operand₂)
+      /--
+      Binary operators applied to two value operands follow the binary operator
+      single-step semantics.
 
+      ### Premises
+
+      - `h₁`: The left-hand operand is a value
+      - `h₂`: The right-hand operand is a value
+      - `h₃`: A single-step binary operation evaluation
+
+      ### Conclusion
+
+      The term evaluates to the result of the binary operation evaluation.
+      -/
       | binOp {op: BinOp} {lhs rhs res: Term} (h₁: IsValue lhs) (h₂: IsValue rhs) (h₃: BinOp.Eval₁ op lhs rhs res): Eval₁ (.binOp op lhs rhs) res
-      | binOpRight {op: BinOp} {lhs rhs₁ rhs₂: Term} (h₁: IsValue lhs) (h₂: Eval₁ rhs₁ rhs₂): Eval₁ (.binOp op lhs rhs₁) (.binOp op lhs rhs₂)
-      | binOpLeft {op: BinOp} {lhs₁ lhs₂ rhs: Term} (h: Eval₁ lhs₁ lhs₂): Eval₁ (.binOp op lhs₁ rhs) (.binOp op lhs₂ rhs)
+      /--
+      Binary operators applied to a value left-hand operand and a non-value
+      right-hand operand evaluate the right-hand operand using the term
+      single-step semantics.
 
+      ### Premises
+
+      - `h₁`: The left-hand operand is a value
+      - `h₂`: A single-step term evaluation of the right-hand operand
+
+      ### Conclusion
+
+      The right-hand operand takes an evaluation step.
+      -/
+      | binOpRight {op: BinOp} {lhs rhs₁ rhs₂: Term} (h₁: IsValue lhs) (h₂: Eval₁ rhs₁ rhs₂): Eval₁ (.binOp op lhs rhs₁) (.binOp op lhs rhs₂)
+      /--
+      Binary operators applied to non-value left- and right-hand operand
+      evaluate the left-hand operand using the term single-step semantics.
+
+      ### Premises
+
+      - `h`: A single-step term evaluation of the left-hand operand
+
+      ### Conclusion
+
+      The left-hand operand takes an evaluation step.
+      -/
+      | binOpLeft {op: BinOp} {lhs₁ lhs₂ rhs: Term} (h: Eval₁ lhs₁ lhs₂): Eval₁ (.binOp op lhs₁ rhs) (.binOp op lhs₂ rhs)
+      /--
+      Conditional expressions with a condition of a literal `true` value
+      evaluate to their `then` expression.
+
+      ### Conclusion
+
+      The conditional evalues to the `then` expression.
+      -/
       | condTrue {t f: Term}: Eval₁ [Term| if tru then ‹t› else ‹f›] [Term| ‹t›]
+      /--
+      Conditional expressions with a condition of a literal `false` value
+      evaluate to their `else` expression.
+
+      ### Conclusion
+
+      The conditional evalues to the `else` expression.
+      -/
       | condFalse {t f: Term}: Eval₁ [Term| if fls then ‹t› else ‹f›] [Term| ‹f›]
+      /--
+      Conditional expressions with a non-value condition expression evaluate the
+      condition expression using the term single-step semantics.
+
+      ### Premises
+
+      - `h`: A single-step term evaluation of the condition expression
+
+      ### Conclusion
+
+      The condition expression takes an evaluation step.
+      -/
       | cond {c₁ c₂ t f: Term} (h: Eval₁ c₁ c₂): Eval₁ [Term| if ‹c₁› then ‹t› else ‹f›] [Term| if ‹c₂› then ‹t› else ‹f›]
 
+    /--
+    ## Multi-Step Evaluation Relation
+
+    The multi-step evaluation relation for terms is the reflexive, transitive
+    closure of the single-step evaluation relation for terms.
+    -/
     abbrev Eval := RTC Eval₁
   end Term
 
   namespace Top
+/-!
+# Top-Level Terms
+-/
+
+    /--
+    ## Value Relation
+
+    TODO: Implement
+    -/
     inductive IsValue: Top → Prop where
+
+    /--
+    ## Typing Relation
+
+    TODO: Implement
+    -/
     inductive HasType: Top → Ty → Prop where
+
+    /--
+    ## Single-Step Evaluation Relation
+
+    TODO: Implement
+    -/
     inductive Eval₁: Top → Top → Prop where
-    def Eval := RTC Eval₁
+
+    /--
+    ## Multi-Step Evalution Relation
+
+    The multi-step evaluation relation for top-level terms is the reflexive,
+    transitive closure of the single-step evaluation relation for top-level
+    terms.
+    -/
+    abbrev Eval := RTC Eval₁
   end Top
+
+  namespace File
+/-!
+# Files
+-/
+  end File
 end Total.Stlc.Lang.Surface
